ported generic acyclicity tools from proof-simplification/BlockInterface.dfy to Graph.dfy

disk-betree/Graph.dfy
@@ -1,4 +1,8 @@
+include "../lib/sequences.dfy"
+  
 abstract module Graph {
+  import opened Sequences
+    
   // Abstract features
   type Reference(!new,==)
   type Node(!new)
@@ -6,7 +10,8 @@ abstract module Graph {
   function Successors(node: Node) : iset<Reference>
 
   type Graph = imap<Reference, Node>
-
+  type Path = seq<Reference>
+    
   // TODO Transactable is a more natural place for this
   datatype Op =
     | AllocOp(ref: Reference, node: Node)
@@ -14,4 +19,115 @@ abstract module Graph {
 
   datatype ReadOp =
     | ReadOp(ref: Reference, node: Node)
+
+  //
+  // Helpers for proving graph-related facts about your data structure.
+  //
+
+  predicate IsClosed(g: Graph) {
+    forall ref :: ref in g ==> Successors(g[ref]) <= g.Keys
+  }
+  
+  predicate IsPath(g: Graph, path: Path) {
+    forall i :: 0 <= i < |path|-1 ==> path[i] in g && path[i+1] in Successors(g[path[i]])
+  }
+
+  predicate IsCycle(g: Graph, path: Path) {
+    && IsPath(g, path)
+    && 0 < |path|
+    && Last(path) in g
+    && path[0] in Successors(g[Last(path)])
+  }
+  
+  predicate IsAcyclic(g: Graph) {
+    forall path :: IsPath(g, path) ==> !IsCycle(g, path)
+  }
+
+  predicate IsPathFromTo(g: Graph, path: Path, start: Reference, end: Reference)
+  {
+    IsPath(g, path) && 1 < |path| && path[0] == start && Last(path) == end
+  }
+  
+  function ReachableReferences(g: Graph, p: Reference) : iset<Reference>
+  {
+    iset path |
+    && IsPath(g, path)
+    && 1 < |path|
+    && path[0] == p
+    :: Last(path)
+  }
+
+  predicate NewPath(g: Graph, g': Graph, p: Reference, path: Path) {
+    && IsPath(g', path)
+    && 1 < |path|
+    && path[0] == p
+    && (forall i :: 0 < i < |path| - 1 ==> path[i] in g'.Keys - g.Keys)
+    && Last(path) in g
+  }
+  
+  function NewlyReachableReferences(g: Graph, g': Graph, p: Reference) : iset<Reference>
+  {
+    iset path | NewPath(g, g', p, path) :: Last(path)
+  }
+
+  predicate EditIsLocal(g: Graph, g': Graph, p: Reference)
+  {
+    && (forall ref :: ref in g.Keys * g'.Keys - iset{p} ==> Successors(g[ref]) == Successors(g'[ref]))
+    && NewlyReachableReferences(g, g', p) <= ReachableReferences(g, p)
+  }
+
+  predicate NewNodesAreCycleFree(g: Graph, g': Graph)
+  {
+    forall path ::
+      && IsPath(g', path)
+      && (forall i :: 0 <= i < |path| ==> path[i] in g'.Keys - g.Keys)
+      ==> !IsCycle(g', path)
+  }
+
+  function FirstInGraph(path: Path, g: Graph) : (pos: int)
+    requires exists i :: 0 <= i < |path| && path[i] in g
+    ensures 0 <= pos < |path|
+    ensures path[pos] in g
+    ensures forall i :: 0 <= i < pos ==> path[i] !in g
+  {
+    if path[0] in g then 0
+    else 1 + FirstInGraph(path[1..], g)
+  }
+
+  function UndoLocalEdit(g: Graph, g': Graph, p: Reference, path: Path) : (result: Path)
+    requires IsClosed(g)
+    requires 1 < |path|
+    requires path[0] in g.Keys
+    requires Last(path) in g.Keys
+    requires EditIsLocal(g, g', p)
+    requires IsPath(g', path)
+    ensures IsPathFromTo(g, result, path[0], Last(path))
+  {
+    if path[0] == p then
+      var len := 1 + FirstInGraph(path[1..], g);
+      var wit := path[..len+1];
+      assert Last(wit) in NewlyReachableReferences(g, g', p);
+      var replacement :| IsPathFromTo(g, replacement, path[0], Last(wit));
+      if len < |path| - 1 then DropLast(replacement) + UndoLocalEdit(g, g', p, path[len..])
+      else replacement
+    else if |path| == 2 then path
+    else path[..1] + UndoLocalEdit(g, g', p, path[1..])
+  }
+  
+  lemma LocalEditPreservesAcyclic(g: Graph, g': Graph, p: Reference)
+    requires IsClosed(g)
+    requires IsAcyclic(g)
+    requires EditIsLocal(g, g', p)
+    requires NewNodesAreCycleFree(g, g')
+    ensures IsAcyclic(g')
+  {
+    if cycle :| IsCycle(g', cycle) {
+      var i :| 0 <= i < |cycle| && cycle[i] in g;
+      var rcycle := cycle[i..] + cycle[..i];
+      assert IsCycle(g', rcycle)  && rcycle[0] in g;
+      var path := rcycle + [rcycle[0]];
+      var rpath := UndoLocalEdit(g, g', p, path);
+      assert IsCycle(g, DropLast(rpath));
+    }
+  }
 }
